RangeSetBlaze.lean
@@ -1,3 +1,7 @@
 -- This module serves as the root of the `RangeSetBlaze` library.
 -- Import modules here that should be built as part of the library.
 import RangeSetBlaze.Basic
+
+-- Export main types and definitions
+export IntRange (toSet isEmpty disjoint isNonEmpty)
+export RangeSetBlaze (toSet checkSortedDisjoint checkNonEmpty)
